A standard Lambda rules also seems to work.

rupicola/stlc/QTyp.fst
@@ -1,52 +1,244 @@
 module QTyp
 
-open FStar.FunctionalExtensionality
+open FStar.Tactics
+open FStar.Classical.Sugar
+open FStar.List.Tot
 
+open STLC
+
+(** We define quotation for Type **)
+
+(** We need quotation for types to define the logical relation. **)
+noeq
+type type_quotation : Type0 -> Type u#1 =
+| QUnit : type_quotation unit
+| QBool : type_quotation bool
+| QArr : #s1:Type ->
+         #s2:Type ->
+         type_quotation s1 ->
+         type_quotation s2 ->
+         type_quotation (s1 -> s2)
+| QPair : #s1:Type ->
+          #s2:Type ->
+          type_quotation s1 ->
+          type_quotation s2 ->
+          type_quotation (s1 & s2)
+| QSum  : #s1:Type ->
+          #s2:Type ->
+          type_quotation s1 ->
+          type_quotation s2 ->
+          type_quotation (either s1 s2)
+
+let test_match s (r:type_quotation s) = (** why does this work so well? **)
+  match r with
+  | QUnit -> assert (s == unit)
+  | QBool -> assert (s == bool)
+  | QArr #s1 #s2 _ _ -> assert (s == (s1 -> s2))
+  | QPair #s1 #s2 _ _ -> assert (s == (s1 & s2))
+  | QSum #s1 #s2 _ _ -> assert (s == either s1 s2)
+
+let rec type_quotation_to_typ #s (r:type_quotation s) : typ =
+  match r with
+  | QUnit -> TUnit
+  | QBool -> TBool
+  | QArr rs1 rs2 -> TArr (type_quotation_to_typ rs1) (type_quotation_to_typ rs2)
+  | QPair rs1 rs2 -> TPair (type_quotation_to_typ rs1) (type_quotation_to_typ rs2)
+  | QSum rs1 rs2 -> TSum (type_quotation_to_typ rs1) (type_quotation_to_typ rs2)
+
+(** Type of Quotable Types **)
+type qType =
+  s:Type & type_quotation s
+
+let pack (q:type_quotation 's) : qType = (| _, q |)
+
+let get_Type (t:qType) = Mkdtuple2?._1 t
+let get_rel (t:qType) = Mkdtuple2?._2 t
+let qUnit : qType = (| _, QUnit |)
+let qBool : qType = (| _, QBool |)
+let (^->) (t1 t2:qType) : qType =
+  (| _, QArr (get_rel t1) (get_rel t2) |)
+
+let (^*) (t1 t2:qType) : qType =
+  (| _, QPair (get_rel t1) (get_rel t2) |)
+let (^+) (t1 t2:qType) : qType =
+  (| _, QSum (get_rel t1) (get_rel t2) |)
+
+(** typ_env is a typing environment: variables to Quotable F* Types **)
+type typ_env = var -> option qType
+let empty : typ_env = fun _ -> None
+
+(* we only need extend at 0 *)
+let extend (t:qType) (g:typ_env)
+  : typ_env
+  = fun y -> if y = 0 then Some t
+          else g (y-1)
+
+let fv_in_env (g:typ_env) (e:exp) : Type0 =
+  forall (fv:var). fv `memP` free_vars e ==> Some? (g fv)
+
+let lem_no_fv_is_closed (e:exp) : Lemma
+  (requires fv_in_env empty e)
+  (ensures is_closed e)
+  [SMTPat (is_closed e)] =
+  ()
+
+let lem_closed_is_no_fv (e:exp) : Lemma
+  (requires is_closed e)
+  (ensures fv_in_env empty e)
+  [SMTPat (is_closed e)] =
+  ()
+
+let lem_fv_in_env_lam (g:typ_env) (t:qType) (body:exp) :
+  Lemma
+    (requires fv_in_env (extend t g) body)
+    (ensures  fv_in_env g (ELam body)) = admit ()
+
+let lem_fv_in_env_app (g:typ_env) (e1 e2:exp) :
+  Lemma
+    (requires fv_in_env g e1 /\ fv_in_env g e2)
+    (ensures  fv_in_env g (EApp e1 e2)) = admit ()
+
+let lem_app_fv_in_env (g:typ_env) (e1 e2:exp) :
+  Lemma
+    (requires fv_in_env g (EApp e1 e2))
+    (ensures fv_in_env g e1 /\ fv_in_env g e2) = admit ()
+
+let lem_fv_in_env_if (g:typ_env) (e1 e2 e3:exp) :
+  Lemma
+    (requires fv_in_env g e1 /\ fv_in_env g e2 /\ fv_in_env g e3)
+    (ensures  fv_in_env g (EIf e1 e2 e3)) = admit ()
+
+let lem_if_fv_in_env (g:typ_env) (e1 e2 e3:exp) :
+  Lemma
+    (requires fv_in_env g (EIf e1 e2 e3))
+    (ensures fv_in_env g e1 /\ fv_in_env g e2 /\ fv_in_env g e3) = admit ()
+
+let lem_fv_in_env_pair (g:typ_env) (e1 e2:exp) :
+  Lemma
+    (requires fv_in_env g e1 /\ fv_in_env g e2)
+    (ensures  fv_in_env g (EPair e1 e2)) = admit ()
+
+let lem_pair_fv_in_env (g:typ_env) (e1 e2:exp) :
+  Lemma
+    (requires fv_in_env g (EPair e1 e2))
+    (ensures fv_in_env g e1 /\ fv_in_env g e2) = admit ()
+
+let lem_fst_fv_in_env (g:typ_env) (e:exp) : // this only makes sense because of how we defined free_vars_indx
+  Lemma
+    (requires fv_in_env g (EFst e))
+    (ensures fv_in_env g e) = admit ()
+
+let lem_snd_fv_in_env (g:typ_env) (e:exp) :
+  Lemma
+    (requires fv_in_env g (ESnd e))
+    (ensures fv_in_env g e) = admit ()
+
+let lem_lam_fv_in_env (g:typ_env) (body:exp) (t1:qType) :
+  Lemma
+    (requires fv_in_env g (ELam body))
+    (ensures fv_in_env (extend t1 g) body) = admit ()
+
+(** STLC Evaluation Environment : variable -> value **)
+let gsub (g:typ_env) (b:bool{b ==> (forall x. None? (g x))}) = (** CA: this b is polluting **)
+  s:(sub b){forall x. Some? (g x) ==> is_value (s x)}
+
+let gsub_empty : gsub empty true =
+  (fun v -> EVar v)
+
+let gsub_extend (#g:typ_env) #b (s:gsub g b) (t:qType) (v:value) : gsub (extend t g) false =
+  let f = fun (y:var) -> if y = 0 then v else s (y-1) in
+  introduce exists (x:var). ~(EVar? (f x)) with 0 and ();
+  f
+
+let gsubst (#g:typ_env) #b (s:gsub g b) (e:exp{fv_in_env g e}) : closed_exp =
+  lem_subst_freevars_closes_exp s e 0;
+  subst s e
+
+let lem_substitution #g #b (s:gsub g b) (t:qType) (v:value) (e:exp)
+  : Lemma (
+    (subst (sub_beta v) (subst (sub_elam s) e)) == (subst (gsub_extend s t v) e))
+  = admit () (** common lemma **)
+
+let lem_gsubst_closed_identiy #g #b (s:gsub g b) (e:closed_exp) :
+  Lemma (gsubst s e == e)
+  [SMTPat (gsubst s e)] =
+  admit ()
+
+module FE = FStar.FunctionalExtensionality
+
+(** eval_env is F* Evaluation Environment : variable -> F* values **)
 type eval_env g =
-  restricted_t (x:var{Some? (g x)}) (fun x -> get_Type (Some?.v (g x)))
-
+  FE.restricted_t (x:var{Some? (g x)}) (fun x -> get_Type (Some?.v (g x)))
 let empty_eval : eval_env empty =
-  on_dom
+  FE.on_dom
     (x:var{Some? (empty x)})
     #(fun x -> get_Type (Some?.v (empty x)))
     (fun _ -> assert False)
-
+val hd : #t:qType -> #g:_ -> eval_env (extend t g) -> get_Type t
 let hd #g fsG = fsG 0
-
+val stack : #g:_ -> fsG:eval_env g -> #t:qType -> get_Type t -> eval_env (extend t g)
 let stack #g fsG #t fs_v =
-  on_dom
+  FE.on_dom
     (x:var{Some? ((extend t g) x)})
     #(fun x -> get_Type (Some?.v ((extend t g) x)))
     (fun y ->
       if y = 0 then fs_v else fsG (y-1))
-
+val tail : #t:qType -> #g:_ -> eval_env (extend t g) -> eval_env g
 let tail #t #g fsG =
-  on_dom
+  FE.on_dom
     (x:var{Some? (g x)})
     #(fun x -> get_Type (Some?.v (g x)))
     (fun y -> fsG (y+1))
-
+val index : #g:_ -> eval_env g -> x:STLC.var{Some? (g x)} -> get_Type (Some?.v (g x))
 let index #g fsG x = fsG x
 
-let lem_stack_hd fsG v = ()
+val lem_hd_stack #t #g (fsG:eval_env g) (v:get_Type t)
+  : Lemma (
+ // (fs_hd fsG == fs_hd (fs_tail (fs_stack fsG v))) /\
+   hd (stack fsG v) == v)
+  [SMTPat (hd (stack fsG v))]
+let lem_hd_stack fsG v = ()
+
+val lem_stack_index #g (fsG:eval_env g) #t (v:get_Type t) : Lemma (
+  (forall (x:var). Some? (g x) ==>  index fsG x == index (stack fsG v) (x+1)) /\
+  index (stack fsG v) 0 == v)
+  [SMTPat (stack fsG v)]
 let lem_stack_index fsG v = ()
+
+val lem_index_tail #g #t (fsG:eval_env (extend t g)) : Lemma (
+  (forall (x:var). Some? (g x) ==>  index fsG (x+1) == index (tail fsG) x))
+  [SMTPat (tail fsG)]
 let lem_index_tail fsG = ()
 
+val tail_stack_inverse #g (fsG:eval_env g) #t (x:get_Type t)
+  : Lemma (tail (stack fsG x) == fsG)
+  [SMTPat (tail (stack fsG x))]
 let tail_stack_inverse #g fsG #t v =
   let fsG' : eval_env g = tail (stack fsG v) in
   assert (forall x. fsG' x == fsG x);
-  assert (feq fsG' fsG);
-  extensionality (x:var{Some? (g x)}) (fun x -> get_Type (Some?.v (g x))) fsG' fsG;
+  assert (FE.feq fsG' fsG);
+  FE.extensionality (x:var{Some? (g x)}) (fun x -> get_Type (Some?.v (g x))) fsG' fsG;
   assert (fsG' == fsG)
 
+val index_0_hd #g #t (fsG:eval_env (extend t g))
+  : Lemma (index fsG 0 == hd fsG)
 let index_0_hd fsG = ()
 
+val lem_stack_tail_hd #g #t (fsG:eval_env (extend t g))
+  : Lemma (stack (tail fsG) (hd fsG) == fsG)
+  [SMTPat (stack (tail fsG) (hd fsG))]
 let lem_stack_tail_hd #g #t fsG =
   let g' : typ_env = extend t g in
   let fsG : eval_env g' = fsG in
   let fsG' : eval_env g' = stack (tail #t #g fsG) (hd #t #g fsG) in
   assert (forall x. fsG' x == fsG x);
-  assert (feq fsG' fsG);
-  extensionality (x:var{Some? (g' x)}) (fun x -> get_Type (Some?.v (g' x))) fsG' fsG;
+  assert (FE.feq fsG' fsG);
+  FE.extensionality (x:var{Some? (g' x)}) (fun x -> get_Type (Some?.v (g' x))) fsG' fsG;
   // TODO: why does this not work?
   assume (fsG' == fsG)
+
+type fs_val (t:qType) =
+  get_Type t
+
+type fs_oval (g:typ_env) (t:qType) =
+  eval_env g -> get_Type t
